Test/dafny0/Parallel.dfy
@@ -2,13 +2,13 @@
 // RUN: %diff "%s.expect" "%t"
 
 class C {
-  var data: int;
-  var n: nat;
-  var st: set<object>;
+  var data: int
+  var n: nat
+  var st: set<object>
 
   ghost method CLemma(k: int)
-    requires k != -23;
-    ensures data < k;  // magic, isn't it (or bogus, some would say)
+    requires k != -23
+    ensures data < k  // magic, isn't it (or bogus, some would say)
 }
 
 // This method more or less just tests the syntax, resolution, and basic verification
@@ -19,31 +19,31 @@ method ParallelStatement_Resolve(
     S: set<int>,
     clx: C, cly: C, clk: int
   )
-  requires a != null && null !in spine;
-  modifies a, spine;
+  requires a != null && null !in spine
+  modifies a, spine
 {
-  forall (i: int | 0 <= i < a.Length && i % 2 == 0) {
+  forall i | 0 <= i < a.Length && i % 2 == 0 {
     a[i] := a[(i + 1) % a.Length] + 3;
   }
 
-  forall (o | o in spine) {
+  forall o | o in spine {
     o.st := o.st + Repr;
   }
 
-  forall (x, y | x in S && 0 <= y+x < 100) {
+  forall x, y | x in S && 0 <= y+x < 100 {
     Lemma(clx, x, y);  // error: precondition does not hold (clx may be null)
   }
 
-  forall (x, y | x in S && 0 <= y+x < 100) {
+  forall x, y | x in S && 0 <= y+x < 100 {
     cly.CLemma(x + y);  // error: receiver might be null
   }
 
-  forall (p | 0 <= p)
-    ensures F(p) <= Sum(p) + p - 1;  // error (no connection is known between F and Sum)
+  forall p | 0 <= p
+    ensures F(p) <= Sum(p) + p - 1  // error (no connection is known between F and Sum)
   {
     assert 0 <= G(p);
     ghost var t;
-    if (p % 2 == 0) {
+    if p % 2 == 0 {
       assert G(p) == F(p+2);  // error (there's nothing that gives any relation between F and G)
       t := p+p;
     } else {
@@ -56,11 +56,11 @@ method ParallelStatement_Resolve(
   }
 }
 
-ghost method Lemma(c: C, x: int, y: int)
-  requires c != null;
-  ensures c.data <= x+y;
-ghost method PowerLemma(x: int, y: int)
-  ensures Pred(x, y);
+lemma Lemma(c: C, x: int, y: int)
+  requires c != null
+  ensures c.data <= x+y
+lemma PowerLemma(x: int, y: int)
+  ensures Pred(x, y)
 
 function F(x: int): int
 function G(x: int): nat
@@ -71,54 +71,54 @@ function Pred(x: int, y: int): bool
 // ---------------------------------------------------------------------
 
 method M0(S: set<C>)
-  requires null !in S;
-  modifies S;
-  ensures forall o :: o in S ==> o.data == 85;
-  ensures forall o :: o != null && o !in S ==> o.data == old(o.data);
+  requires null !in S
+  modifies S
+  ensures forall o :: o in S ==> o.data == 85
+  ensures forall o :: o != null && o !in S ==> o.data == old(o.data)
 {
-  forall (s | s in S) {
+  forall s | s in S {
     s.data := 85;
   }
 }
 
 method M1(S: set<C>, x: C)
-  requires null !in S && x in S;
+  requires null !in S && x in S
 {
-  forall (s | s in S)
-    ensures s.data < 100;
+  forall s | s in S
+    ensures s.data < 100
   {
     assume s.data == 85;
   }
-  if (*) {
+  if * {
     assert x.data == 85;  // error (cannot be inferred from forall ensures clause)
   } else {
     assert x.data < 120;
   }
 
-  forall (s | s in S)
-    ensures s.data < 70;  // error
+  forall s | s in S
+    ensures s.data < 70  // error
   {
     assume s.data == 85;
   }
 }
 
 method M2() returns (a: array<int>)
-  ensures a != null;
-  ensures forall i,j :: 0 <= i < a.Length/2 <= j < a.Length ==> a[i] < a[j];
+  ensures a != null
+  ensures forall i,j :: 0 <= i < a.Length/2 <= j < a.Length ==> a[i] < a[j]
 {
   a := new int[250];
-  forall (i: nat | i < 125) {
+  forall i: nat | i < 125 {
     a[i] := 423;
   }
-  forall (i | 125 <= i < 250) {
+  forall i | 125 <= i < 250 {
     a[i] := 300 + i;
   }
 }
 
 method M4(S: set<C>, k: int)
-  modifies S;
+  modifies S
 {
-  forall (s | s in S && s != null) {
+  forall s | s in S && s != null {
     s.n := k;  // error: k might be negative
   }
 }
@@ -127,25 +127,25 @@ method M5()
 {
   if {
   case true =>
-    forall (x | 0 <= x < 100) {
+    forall x | 0 <= x < 100 {
       PowerLemma(x, x);
     }
     assert Pred(34, 34);
 
   case true =>
-    forall (x,y | 0 <= x < 100 && y == x+1) {
+    forall x,y | 0 <= x < 100 && y == x+1 {
       PowerLemma(x, y);
     }
     assert Pred(34, 35);
 
   case true =>
-    forall (x,y | 0 <= x < y < 100) {
+    forall x,y | 0 <= x < y < 100 {
       PowerLemma(x, y);
     }
     assert Pred(34, 35);
 
   case true =>
-    forall (x | x in set k | 0 <= k < 100) {
+    forall x | x in set k | 0 <= k < 100 {
       PowerLemma(x, x);
     }
     assert Pred(34, 34);
@@ -155,22 +155,22 @@ method M5()
 method Main()
 {
   var a := new int[180];
-  forall (i | 0 <= i < 180) {
+  forall i | 0 <= i < 180 {
     a[i] := 2*i + 100;
   }
   var sq := [0, 0, 0, 2, 2, 2, 5, 5, 5];
-  forall (i | 0 <= i < |sq|) {
+  forall i | 0 <= i < |sq| {
     a[20+i] := sq[i];
   }
-  forall (t | t in sq) {
+  forall t | t in sq {
     a[t] := 1000;
   }
-  forall (t,u | t in sq && t < 4 && 10 <= u < 10+t) {
+  forall t,u | t in sq && t < 4 && 10 <= u < 10+t {
     a[u] := 6000 + t;
   }
   var k := 0;
-  while (k < 180) {
-    if (k != 0) { print ", "; }
+  while k < 180 {
+    if k != 0 { print ", "; }
     print a[k];
     k := k + 1;
   }
@@ -180,50 +180,50 @@ method Main()
 method DuplicateUpdate() {
   var a := new int[180];
   var sq := [0, 0, 0, 2, 2, 2, 5, 5, 5];
-  if (*) {
-    forall (t,u | t in sq && 10 <= u < 10+t) {
+  if * {
+    forall t,u | t in sq && 10 <= u < 10+t {
       a[u] := 6000 + t;  // error: a[10] (and a[11]) are assigned more than once
     }
   } else {
-    forall (t,u | t in sq && t < 4 && 10 <= u < 10+t) {
+    forall t,u | t in sq && t < 4 && 10 <= u < 10+t {
       a[u] := 6000 + t;  // with the 't < 4' conjunct in the line above, this is fine
     }
   }
 }
 
-ghost method DontDoMuch(x: int)
+lemma DontDoMuch(x: int)
 {
 }
 
 method OmittedRange() {
-  forall (x: int) { }  // a type is still needed for the bound variable
-  forall (x) {
+  forall x: int { }  // a type is still needed for the bound variable
+  forall x {
     DontDoMuch(x);
   }
 }
 
 // ----------------------- two-state postconditions ---------------------------------
 
-class TwoState_C { ghost var data: int; }
+class TwoState_C { ghost var data: int }
 
 // It is not possible to achieve this postcondition in a ghost method, because ghost
 // contexts are not allowed to allocate state.  Callers of this ghost method will know
 // that the postcondition is tantamount to 'false'.
 ghost method TwoState0(y: int)
-  ensures exists o: TwoState_C :: o != null && fresh(o);
+  ensures exists o: TwoState_C :: o != null && fresh(o)
 
 method TwoState_Main0() {
-  forall (x) { TwoState0(x); }
+  forall x { TwoState0(x); }
   assert false;  // no prob, because the postcondition of TwoState0 implies false
 }
 
 method X_Legit(c: TwoState_C)
-  requires c != null;
-  modifies c;
+  requires c != null
+  modifies c
 {
   c.data := c.data + 1;
-  forall (x | c.data <= x)
-    ensures old(c.data) < x;  // note that the 'old' refers to the method's initial state
+  forall x | c.data <= x
+    ensures old(c.data) < x  // note that the 'old' refers to the method's initial state
   {
   }
 }
@@ -235,8 +235,8 @@ method X_Legit(c: TwoState_C)
 // method, not the beginning of the 'forall' statement.
 method TwoState_Main2()
 {
-  forall (x: int)
-    ensures exists o: TwoState_C :: o != null && fresh(o);
+  forall x: int
+    ensures exists o: TwoState_C :: o != null && fresh(o)
   {
     TwoState0(x);
   }
@@ -251,8 +251,8 @@ method TwoState_Main2()
 // statement's effect on the heap is not optimized away.
 method TwoState_Main3()
 {
-  forall (x: int)
-    ensures exists o: TwoState_C :: o != null && fresh(o);
+  forall x: int
+    ensures exists o: TwoState_C :: o != null && fresh(o)
   {
     assume false;  // (there's no other way to achieve this forall-statement postcondition)
   }
@@ -262,11 +262,11 @@ method TwoState_Main3()
 // ------- empty forall statement -----------------------------------------
 
 class EmptyForallStatement {
-  var emptyPar: int;
+  var emptyPar: int
 
   method Empty_Parallel0()
-    modifies this;
-    ensures emptyPar == 8;
+    modifies this
+    ensures emptyPar == 8
   {
     forall () {
       this.emptyPar := 8;
@@ -274,11 +274,11 @@ class EmptyForallStatement {
   }
 
   function EmptyPar_P(x: int): bool
-  ghost method EmptyPar_Lemma(x: int)
-    ensures EmptyPar_P(x);
+  lemma EmptyPar_Lemma(x: int)
+    ensures EmptyPar_P(x)
 
   method Empty_Parallel1()
-    ensures EmptyPar_P(8);
+    ensures EmptyPar_P(8)
   {
     forall {
       EmptyPar_Lemma(8);
@@ -288,7 +288,7 @@ class EmptyForallStatement {
   method Empty_Parallel2()
   {
     forall
-      ensures exists k :: EmptyPar_P(k);
+      ensures exists k :: EmptyPar_P(k)
     {
       var y := 8;
       assume EmptyPar_P(y);
@@ -312,9 +312,9 @@ predicate ThProperty(step: nat, t: Nat, r: nat)
   case Succ(o) => step>0 && exists ro:nat :: ThProperty(step-1, o, ro)
 }
 
-ghost method Th(step: nat, t: Nat, r: nat)
-  requires t.Succ? && ThProperty(step, t, r);
+lemma Th(step: nat, t: Nat, r: nat)
+  requires t.Succ? && ThProperty(step, t, r)
   // the next line follows from the precondition and the definition of ThProperty
-  ensures exists ro:nat :: ThProperty(step-1, t.tail, ro);
+  ensures exists ro:nat :: ThProperty(step-1, t.tail, ro)
 {
 }
